Prove common closeable chan pattern (in which no send operations occur
on a channel). Frequently used for signaling in etcd code.
More improvement to chan.select spec

new/golang/theory/chan.v
@@ -37,7 +37,7 @@ Arguments is_chan {_ _ _ _ _ _} (_) {_} ch.
 
 Section proof.
 Context `{hG: heapGS Σ, !ffi_semantics _ _}.
-Context `{!IntoVal V, !IntoValTyped V t}.
+Context `{!IntoVal V}.
 
 Implicit Types v : V.
 Implicit Types (s : chanstate.t V).
@@ -52,14 +52,14 @@ Lemma is_chan_not_nil ch :
 Proof.
 Admitted.
 
-Lemma wp_chan_make cap :
+Lemma wp_chan_make `{!IntoValTyped V t} cap :
   {{{ True }}}
     chan.make t #cap
   {{{ (c : chan.t) (init : list V), RET #c; own_chan c (chanstate.mk cap false init (length init)) }}}.
 Proof.
 Admitted.
 
-Definition receive_atomic_update ch Φ : iProp Σ :=
+Definition receive_atomic_update `{!IntoValTyped V t} ch Φ : iProp Σ :=
   |={⊤,∅}=>
     ▷∃ s, own_chan ch s ∗
           if decide (s.(chanstate.closed) = true ∧ s.(chanstate.received) = length s.(chanstate.sent)) then
@@ -74,7 +74,7 @@ Definition receive_atomic_update ch Φ : iProp Σ :=
                            (∀ v, ⌜ s'.(chanstate.sent) !! s.(chanstate.received) = Some v ⌝ -∗
                                  own_chan ch s' ={∅,⊤}=∗ Φ (#v, #true)%V))).
 
-Lemma wp_chan_receive ch :
+Lemma wp_chan_receive `{!IntoValTyped V t} ch :
   ∀ Φ,
   is_chan V ch -∗
   ▷ receive_atomic_update ch Φ -∗
@@ -141,7 +141,7 @@ Lemma wp_for_chan_range P ch (body : func.t) :
                             own_chan ch s' ={∅,⊤}=∗ WP #body #v {{ for_chan_postcondition P Φ }})))
     ) -∗
   WP chan.for_range #ch #body {{ Φ }}.
-Proof using IntoValTyped0.
+Proof.
 Admitted.
 
 Lemma wp_for_chan_post_do (v : val) P Φ :
@@ -182,10 +182,10 @@ End proof.
     current context to the loop invariant, then apply this tactic. Use
     [wp_for_chan_post] for the leaves of the proof. *)
 Ltac wp_for_chan_core :=
-  wp_bind (chan.for_range _ _); (iApply (wp_for_chan_range (IntoValTyped0:=?[ivt]) with "[-]"));
+  wp_bind (chan.for_range _ _); (iApply (wp_for_chan_range with "[-]"));
   [ by iNamedAccu
   | (by iFrame "#" || fail "wp_for_chan_core: could not solve [is_chan] by [iFrame ""#""]. ")
-  | iIntros "!# __CTX"; iNamed "__CTX" ]; instantiate(ivt:=ltac:(tc_solve)).
+  | iIntros "!# __CTX"; iNamed "__CTX" ].
 
 
 (** Automatically apply the right theorem for [for_chan_postcondition] *)
@@ -245,9 +245,8 @@ Context `{hG: heapGS Σ, !ffi_semantics _ _}.
 
 Lemma wp_chan_select_blocking (cases : list chan.op) :
   ∀ Φ,
-  (∀ idx op,
-     ⌜ cases !! idx = Some op ⌝ →
-     match op with
+  ([∧ list] case ∈ cases,
+     match case with
      | chan.select_send_f send_val send_chan send_handler =>
          (∃ V (v : V) `(!IntoVal V),
              ⌜ send_val = #v ⌝ ∗
@@ -264,163 +263,3 @@ Proof.
 Admitted.
 
 End select_proof.
-
-Section onetime_barrier.
-Context `{hG: heapGS Σ, !ffi_semantics _ _}.
-Context `{!ghost_varG Σ ()}.
-
-Implicit Types (s : chanstate.t unit).
-
-Record params :=
-  {
-    gauge_init : nat; (* XXX: putting "gauge" in the name because this would
-                       change under a `chan` gauge transformation. *)
-    send_gn : gname;
-    recv_gn : gname;
-  }.
-Implicit Types γ : params.
-
-Definition own_send_tok γ := ghost_var γ.(send_gn) 1 ().
-Definition own_recv_tok γ := ghost_var γ.(recv_gn) 1 ().
-
-Definition is_onetime_barrier γ (ch : chan.t) Sd Rv : iProp Σ :=
-  is_chan () ch ∗
-  inv nroot (
-      ∃ s,
-        "Hch" ∷ own_chan ch s ∗
-        "%Hcap" ∷ ⌜ s.(chanstate.cap) = W64 0 ⌝ ∗
-        "%Hopen" ∷ ⌜ s.(chanstate.closed) = false ⌝ ∗
-        "%Hoffset_r" ∷ ⌜ γ.(gauge_init) ≤ s.(chanstate.received) ⌝%nat ∗
-        "%Hoffset_s" ∷ ⌜ γ.(gauge_init) ≤ length s.(chanstate.sent) ⌝%nat ∗
-        "Hr" ∷ match (s.(chanstate.received) - γ.(gauge_init))%nat with
-          | O => True
-          | S _ => (Rv ∨ own_send_tok γ)
-          end ∗
-        "Hs" ∷ match (length s.(chanstate.sent) - γ.(gauge_init))%nat with
-          | O => True
-          | S _ => (Sd ∨ own_recv_tok γ)
-          end
-    ).
-
-Lemma start_onetime_barrier Sd Rv ch s:
-  s.(chanstate.cap) = (W64 0) →
-  s.(chanstate.closed) = false →
-  s.(chanstate.received) = length s.(chanstate.sent) →
-  is_chan () ch -∗
-  own_chan ch s ={⊤}=∗
-  ∃ γ, is_onetime_barrier γ ch Sd Rv ∗
-       own_recv_tok γ ∗
-       own_send_tok γ.
-Proof.
-  intros.
-  iIntros "#? Hchan".
-  iMod (ghost_var_alloc ()) as "[% ?]".
-  iMod (ghost_var_alloc ()) as "[% ?]".
-  iExists _.
-  instantiate (1:=(ltac:(econstructor))). simpl.
-  iFrame "#". iFrame. simpl.
-  iApply inv_alloc.
-  iNext. iFrame "∗%".
-  instantiate (1:=s.(chanstate.received)).
-  iSplitR; first word.
-  iSplitR; first word.
-  rewrite H1 Nat.sub_diag //.
-Qed.
-
-Lemma wp_onetime_barrier_receive γ ch Sd Rv :
-  {{{
-      is_onetime_barrier γ ch Sd Rv ∗
-      own_recv_tok γ ∗
-      Rv
-  }}}
-    chan.receive #ch
-  {{{
-      RET (#(), #true); Sd
-  }}}.
-Proof.
-  iIntros (?) "((#Hchan & #Hinv) & Htok & HR) HΦ".
-  wp_apply (wp_chan_receive (V:=()) with "[$]").
-
-  (* send Rv *)
-  iInv "Hinv" as "Hi" "Hclose".
-  iApply fupd_mask_intro; [set_solver | iIntros "Hmask"].
-  iNext. iNamed "Hi".
-  iExists _; iFrame.
-  rewrite Hopen.
-  iIntros "Hch".
-  iMod "Hmask" as "_".
-  iMod ("Hclose" with "[-Htok HΦ]").
-  { iNext. iFrame "∗%".
-    simpl. iSplitR; first word.
-    rewrite Nat.sub_succ_l //. iFrame.
-  }
-  iModIntro.
-
-  (* get Sd *)
-  iInv "Hinv" as "Hi" "Hclose".
-  iApply fupd_mask_intro; [set_solver | iIntros "Hmask"].
-  iNext. iNamed "Hi".
-  iExists _; iFrame.
-  iIntros "* % Hch".
-
-  edestruct (length _ - _)%nat eqn:?.
-  { simpl in *. exfalso. apply lookup_lt_Some in H. lia. }
-  iDestruct "Hs" as "[Hs|Hbad]".
-  2:{ iCombine "Hbad Htok" gives %[Hbad _]. done. }
-  iMod "Hmask" as "_".
-  iMod ("Hclose" with "[-HΦ Hs]").
-  { iNext. iFrame "∗%". destruct (_ - _)%nat; iFrame. }
-  iModIntro.
-  destruct v.
-  iApply "HΦ".
-  iFrame.
-Qed.
-
-Lemma wp_onetime_barrier_send γ ch Sd Rv :
-  {{{
-      is_onetime_barrier γ ch Sd Rv ∗
-      own_send_tok γ ∗
-      Sd
-  }}}
-    chan.send #ch #()
-  {{{
-      RET #(); Rv
-  }}}.
-Proof.
-  iIntros (?) "((#Hchan & #Hinv) & Htok & HR) HΦ".
-  wp_apply (wp_chan_send (V:=()) with "[$]").
-
-  (* send Sd *)
-  iInv "Hinv" as "Hi" "Hclose".
-  iApply fupd_mask_intro; [set_solver | iIntros "Hmask"].
-  iNext. iNamed "Hi".
-  iExists _; iFrame "∗%".
-  iIntros "Hch".
-  iMod "Hmask" as "_".
-  iMod ("Hclose" with "[-Htok HΦ]").
-  { iNext. iFrame "∗%". iSplitR.
-    { rewrite length_app /=. iPureIntro. lia. }
-    iClear "Hs". by destruct Nat.sub; iFrame.
-  }
-  iModIntro.
-
-  (* get Rv *)
-  iInv "Hinv" as "Hi" "Hclose".
-  iApply fupd_mask_intro; [set_solver | iIntros "Hmask"].
-  iNext. iNamed "Hi".
-  iExists _; iFrame.
-  iIntros "* % Hch".
-
-  edestruct (chanstate.received s0 - _)%nat eqn:?.
-  { simpl in *. exfalso. word. }
-  iDestruct "Hr" as "[Hr|Hbad]".
-  2:{ iCombine "Hbad Htok" gives %[Hbad _]. done. }
-  iMod "Hmask" as "_".
-  iMod ("Hclose" with "[-HΦ Hr]").
-  { iNext. iFrame "∗%". by destruct Nat.sub; iFrame. }
-  iModIntro.
-  iApply "HΦ".
-  iFrame.
-Qed.
-
-End onetime_barrier.
