new/proof/chan_proof/closeable.v
@@ -1,0 +1,97 @@
+Require Import New.proof.proof_prelude.
+
+(** A pattern for channel usage: a channel that never has anything sent, and is
+    only closed at some point. Closing transfers a persistent proposition to
+    readers. *)
+Class closeable_chanG Σ :=
+  {
+    ghost_varG :: ghost_varG Σ ()
+  }.
+
+Record closeable_chan_names :=
+  {
+    tok_gn : gname;
+    init_len : nat; (* for gauge invariance *)
+  }.
+
+Section proof.
+
+Context `{hG: heapGS Σ, !ffi_semantics _ _}.
+Context `{closeable_chanG Σ}.
+
+Local Definition own_closeable_chan γch : iProp Σ :=
+  ghost_var γch.(tok_gn) 1 ().
+
+(* Note: could make the namespace be user-chosen *)
+Definition is_closeable_chan V `{!IntoVal V} (ch : chan.t) γch (Pclose : iProp Σ) : iProp Σ :=
+  "#His_ch" ∷ is_chan V ch ∗
+  "#Hinv" ∷ inv nroot (
+      ∃ (st : chanstate.t V),
+        "ch" ∷ own_chan ch st ∗
+        "%Hempty" ∷ ⌜ length st.(chanstate.sent) = γch.(init_len) ⌝ ∗
+        "%Hle" ∷ ⌜ length st.(chanstate.sent) ≤ st.(chanstate.received) ⌝ ∗
+        "#HPclosed" ∷ (if st.(chanstate.closed) then (□ Pclose) else True) ∗
+        "Hclosed" ∷ (if st.(chanstate.closed) then own_closeable_chan γch else True)
+    ).
+#[global] Opaque is_closeable_chan.
+#[local] Transparent is_closeable_chan.
+#[global] Instance is_closeable_chan_pers V `{!IntoVal V} γch ch P :
+  Persistent (is_closeable_chan V γch ch P) := _.
+
+Context `{!IntoVal V}.
+Context `{!IntoValTyped V t}.
+Lemma closeable_chan_receive ch γch Pclosed Φ :
+  is_closeable_chan V ch γch Pclosed -∗
+  (Pclosed -∗ Φ (#(default_val V), #false)%V) -∗ receive_atomic_update ch Φ (V:=V).
+Proof.
+  iNamed 1. iIntros "HΦ". rewrite /receive_atomic_update.
+  iInv "Hinv" as "Hi" "Hclose". iApply fupd_mask_intro; [ solve_ndisj | iIntros "Hmask"].
+  iNext. iNamed "Hi". iFrame.
+  destruct decide as [|].
+  - iIntros "Hch". iFrame.
+    iMod "Hmask" as "_". iMod ("Hclose" with "[-HΦ]").
+    { iFrame "∗#%". } iApply "HΦ". destruct st.(chanstate.closed); try done.
+    naive_solver.
+  - (* eventually get a contradiction down this path *)
+    iIntros "Hch". iMod "Hmask" as "_".
+    iMod ("Hclose" with "[-]"). { iFrame "∗#%". iPureIntro. simpl. lia. }
+    iModIntro.
+    iInv "Hinv" as "Hi" "Hclose". iApply fupd_mask_intro; [ solve_ndisj | iIntros "Hmask"].
+    iNext. iNamed "Hi". iFrame. iIntros (?) "%Hbad".
+    exfalso. apply lookup_lt_Some in Hbad. lia.
+Qed.
+
+Lemma wp_closeable_chan_close ch γch Pclosed Φ :
+  is_closeable_chan V ch γch Pclosed ∗ own_closeable_chan γch ∗ □ Pclosed -∗
+  Φ #() -∗
+  WP chan.close #ch {{ Φ }}.
+Proof.
+  iIntros "(#His & Hown & #HP) HΦ". iNamed "His".
+  unshelve wp_apply (wp_chan_close with "[$]"); try tc_solve.
+  iInv "Hinv" as "Hi" "Hclose". iApply fupd_mask_intro; [ solve_ndisj | iIntros "Hmask"].
+  iNext. iNamed "Hi". iFrame. destruct (st.(chanstate.closed)).
+  { iCombine "Hown Hclosed" gives %Hbad. exfalso. naive_solver. }
+  iSplitR; first done. iIntros "Hch". iMod "Hmask" as "_".
+  iMod ("Hclose" with "[-]"); last done.
+  iFrame "∗#%".
+Qed.
+
+Lemma alloc_closeable_chan {E} Pclose ch (s : chanstate.t V) :
+  s.(chanstate.received) = length s.(chanstate.sent) →
+  s.(chanstate.closed) = false →
+  is_chan V ch -∗
+  own_chan ch s ={E}=∗
+  ∃ γch,
+  is_closeable_chan V ch γch Pclose ∗
+  own_closeable_chan γch.
+Proof.
+  intros ? Hnotclosed. iIntros "His Hch".
+  iMod (ghost_var_alloc ()) as (tok_gn) "Htok".
+  iExists _. instantiate (1:=ltac:(econstructor)).
+  simpl. iFrame.
+  iMod (inv_alloc with "[-]") as "$"; last done.
+  iFrame. rewrite Hnotclosed. simpl.
+  iPureIntro. split; [done|lia].
+Qed.
+
+End proof.
